lib/Lib.Buffer.fsti
@@ -42,6 +42,33 @@ unfold let ibuffer (a:Type0) = buffer_t IMMUT a
 (** Const buffer. Either one of the two above. Extracts as `const a*`. *)
 unfold let cbuffer (a:Type0) = buffer_t CONST a
 
+let pre #ty #a (b: buffer_t ty a) =
+  match ty with
+  | IMMUT -> IB.immutable_preorder a
+  | MUT -> B.trivial_preorder a
+  | CONST -> CB.(qbuf_pre (as_qbuf (b <: CB.const_buffer a)))
+
+(* Usable only from functions marked themselves as inline_for_extraction, or
+  applied to a constant ty (must reduce). This may generate a cast. Only for
+  compatibility purposes as we migrate code to const, but still need to call code
+  that hasn't been const-ified. *)
+inline_for_extraction
+let as_mbuf #ty #a (b: buffer_t ty a): LMB.mbuffer a (pre b) (pre b) =
+  match ty with
+  | IMMUT -> b
+  | MUT -> b
+  | CONST -> CB.cast b
+
+(* Usable only from functions marked themselves as inline_for_extraction, or
+  applied to a constant ty (must reduce). Doesn't generate a cast (const
+  conversion is implicit in C.) *)
+inline_for_extraction
+let as_cbuf #ty #a (b: buffer_t ty a): CB.const_buffer a =
+  match ty with
+  | IMMUT -> CB.of_ibuffer b
+  | MUT -> CB.of_buffer b
+  | CONST -> b
+
 let length (#t:buftype) (#a:Type0) (b:buffer_t t a) =
   match t with
   | MUT -> B.length (b <: buffer a)
